tweak bvl_bc_table and prove more about it
make it insert the jump that jumps over the code table, and show that
this jump works (as well as showing that the code table is good).

new-backend/bvlBytecodeScript.sml
@@ -2666,7 +2666,10 @@ val bvl_bc_ptrfun_correct = prove(
       ⇒
       let (f,s) = FOLDR (UNCURRY (bvl_bc_ptrfun il)) (f0,s0) ls in
         ALL_DISTINCT (FILTER is_Label s.out) ∧
-        EVERY (combin$C $< s.next_label o dest_Label) (FILTER is_Label s.out) ∧
+        (∃code.
+           code ++ s0.out = s.out ∧
+           EVERY (between s0.next_label s.next_label o dest_Label) (FILTER is_Label code) ∧
+           s0.next_label ≤ s.next_label) ∧
         ∀ptr exp arity.
           MEM (ptr,(arity,exp)) ls ⇒
             ∃cs l0 cc l1.
@@ -2682,12 +2685,17 @@ val bvl_bc_ptrfun_correct = prove(
   simp[bvl_bc_ptrfun_def] >>
   simp[PULL_FORALL] >> rpt gen_tac >>
   specl_args_of_then``bvl_bc``bvl_bc_append_out strip_assume_tac >>
-  ONCE_REWRITE_TAC[CONJ_ASSOC] >>
   conj_tac >- (
+    qpat_assum`X = r.out`(assume_tac o SYM) >>
     fs[FILTER_APPEND,ALL_DISTINCT_APPEND] >>
     fs[EVERY_MEM,MEM_MAP,PULL_EXISTS,MEM_FILTER,is_Label_rwt,between_def] >>
     rw[]>>res_tac>>rfs[]>>spose_not_then strip_assume_tac>>fsrw_tac[ARITH_ss][]>>
     res_tac>>fsrw_tac[ARITH_ss][]) >>
+  conj_tac >- (
+    qpat_assum`X = r.out`(assume_tac o SYM) >> simp[] >>
+    fs[EVERY_MEM,between_def,MEM_MAP,PULL_EXISTS,FILTER_APPEND] >>
+    fs[MEM_FILTER,is_Label_rwt,PULL_EXISTS] >> rw[] >> simp[] >>
+    res_tac >> fsrw_tac[ARITH_ss][] ) >>
   reverse strip_tac >- (
     res_tac >>
     first_assum(match_exists_tac o concl) >> simp[] >>
@@ -2700,7 +2708,10 @@ val bvl_bc_ptrfun_correct = prove(
   qexists_tac`r`>> fs[] >>
   simp[tlookup_def] >>
   qexists_tac`REVERSE r.out`>>simp[] >>
-  simp[FILTER_REVERSE,ALL_DISTINCT_REVERSE,EVERY_REVERSE])
+  simp[FILTER_REVERSE,ALL_DISTINCT_REVERSE,EVERY_REVERSE] >>
+  qpat_assum`X = r.out`(assume_tac o SYM) >>
+  fs[EVERY_MEM,MEM_FILTER,is_Label_rwt,PULL_EXISTS,between_def,MEM_MAP] >>
+  rw[] >> res_tac >> fsrw_tac[ARITH_ss][])
   |> Q.GENL[`s0`,`f0`]
 
 val update_ptr_def = Define`
@@ -2857,8 +2868,8 @@ val bvl_bc_update_ptr = store_thm("bvl_bc_update_ptr",
 
 val bvl_bc_table_def = Define`
   bvl_bc_table il nl cmap =
-    let (f,s) = foldi (bvl_bc_ptrfun il) 0 (LN, <|next_label:=nl;out:=[]|>) cmap in
-    (f,s with out := MAP (update_ptr f) s.out)`
+    let (f,s) = foldi (bvl_bc_ptrfun il) 0 (LN, <|next_label:=nl+1;out:=[Jump(Lab nl)]|>) cmap in
+    (f,s with out := (Label nl)::(MAP (update_ptr f) s.out))`
 
 val is_Label_o_update_ptr = prove(
   ``is_Label o (update_ptr f) = is_Label``,
@@ -2880,12 +2891,12 @@ val next_addr_MAP_update_ptr = prove(
   Cases_on`l`>>simp[] >>
   fs[bytecodeLabelsTheory.length_ok_def])
 
-val bvl_bc_table_correct = store_thm("bvl_bc_table_correct",
+val bvl_bc_table_good = store_thm("bvl_bc_table_good",
   ``length_ok il ⇒
     bvl_bc_table il nl cmap = (f,s) ⇒
     good_code_env f il cmap (REVERSE s.out)``,
   rw[bvl_bc_table_def,foldi_FOLDR_toAList] >>
-  qspecl_then[`LN`,`<|next_label := nl; out:=[]|>`,`toAList cmap`]mp_tac
+  qspecl_then[`LN`,`<|next_label := nl+1; out:=[Jump(Lab nl)]|>`,`toAList cmap`]mp_tac
     (INST_TYPE[alpha|->numSyntax.num] bvl_bc_ptrfun_correct) >>
   discharge_hyps >- (
     simp[ALL_DISTINCT_MAP_FST_toAList] ) >>
@@ -2903,5 +2914,38 @@ val bvl_bc_table_correct = store_thm("bvl_bc_table_correct",
   simp[GSYM MAP_REVERSE] >>
   simp[FILTER_is_Label_MAP_update_ptr] >>
   simp[next_addr_MAP_update_ptr])
+
+val bvl_bc_table_thm = store_thm("bvl_bc_table_thm",
+  ``bvl_bc_table il nl cmap = (f,s) ⇒
+    ∀bs bc0 bc1.
+    ALL_DISTINCT (FILTER is_Label bc0) ∧
+    EVERY ($> nl o dest_Label) (FILTER is_Label bc0) ∧
+    bs.code = bc0 ++ REVERSE s.out ++ bc1 ∧
+    bs.pc = next_addr bs.inst_length bc0 ⇒
+    bc_next bs (bs with <|pc := next_addr bs.inst_length (bc0++REVERSE s.out)|>)``,
+  rw[bvl_bc_table_def,foldi_FOLDR_toAList] >>
+  qspecl_then[`LN`,`<|next_label := nl+1; out:=[Jump(Lab nl)]|>`,`toAList cmap`]mp_tac
+    (INST_TYPE[alpha|->numSyntax.num] bvl_bc_ptrfun_correct) >>
+  discharge_hyps >- (
+    simp[ALL_DISTINCT_MAP_FST_toAList] ) >>
+  fs[LET_THM] >>
+  first_assum (split_applied_pair_tac o lhs o concl) >>
+  fs[] >> rw[] >>
+  `bc_fetch bs = SOME(Jump(Lab nl))` by (
+    qpat_assum`X = Y.out`(assume_tac o SYM) >> fs[] >>
+    match_mp_tac bc_fetch_next_addr >>
+    qexists_tac`bc0`>>simp[] ) >>
+  simp[bc_eval1_thm,bc_eval1_def] >>
+  simp[bc_state_component_equality] >>
+  simp[bc_find_loc_def] >>
+  match_mp_tac bc_find_loc_aux_append_code >>
+  match_mp_tac bc_find_loc_aux_ALL_DISTINCT >>
+  qexists_tac`LENGTH bc0 + LENGTH s'.out` >>
+  simp[EL_APPEND1,EL_APPEND2,TAKE_APPEND2,TAKE_APPEND1] >>
+  simp[SUM_APPEND,FILTER_APPEND,SUM_REVERSE,FILTER_REVERSE,MAP_REVERSE] >>
+  simp[ALL_DISTINCT_APPEND,ALL_DISTINCT_REVERSE,FILTER_is_Label_MAP_update_ptr] >>
+  fs[ALL_DISTINCT_APPEND,FILTER_APPEND,MEM_FILTER,is_Label_rwt,PULL_EXISTS,EVERY_MEM] >>
+  qpat_assum`X = Y.out`(assume_tac o SYM) >> fs[between_def,FILTER_APPEND,ALL_DISTINCT_APPEND] >>
+  rw[] >> spose_not_then strip_assume_tac >> res_tac >> fsrw_tac[ARITH_ss][])
 
 val _ = export_theory()
